queue: also prove invoc-based spec for push

misc/queue.bpl
@@ -150,6 +150,16 @@ axiom (forall s: SeqInvoc, n: Invoc :: {Queue.ofSeq(Seq_append(s, n))}
   && Queue.stateArray(Queue.ofSeq(Seq_append(s, n)))
     == Queue.stateArray(Queue.ofSeq(s)));
 
+axiom (forall s: SeqInvoc, n: Invoc :: {Queue.ofSeq(Seq_append(s, n))}
+  invoc_m(n) == Queue.push
+  ==> Queue.stateHead(Queue.ofSeq(Seq_append(s, n)))
+    == Queue.stateHead(Queue.ofSeq(s))
+  && Queue.stateTail(Queue.ofSeq(Seq_append(s, n)))
+    == Queue.stateTail(Queue.ofSeq(s)) + 1
+  && Queue.stateArray(Queue.ofSeq(Seq_append(s, n)))
+    == Queue.stateArray(Queue.ofSeq(s))[
+      Queue.stateTail(Queue.ofSeq(Seq_append(s, n))) := invoc_k(n)]);
+
 
 // ---------- Representation of execution and linearization
 
@@ -296,7 +306,7 @@ var {:layer 0, 1} start: Ref; // The first head. To define usedFP
 
 
 // Abstract state
-var {:layer 1,2} absRefs: [int]Ref;  // connection between abstract and concrete
+var {:layer 1,1} absRefs: [int]Ref;  // connection between abstract and concrete
 
 
 function {:inline} Inv(queueFP: [Ref]bool, usedFP: [Ref]bool, start: Ref,
@@ -429,23 +439,11 @@ procedure {:yields} {:layer 0} {:refines "casHeadTransfer_atomic"}
 
 // ---------- Primitives for manipulating logical/abstract state
 
-// procedure {:layer 1} {:inline 1} intro_writeAbs(k: Key, x: Ref)
-//   modifies absRefs;
-// {
-//   absRefs[absTail] := x;
-// }
-
-// procedure {:layer 1} {:inline 1} intro_incrHead()
-//   modifies absHead;
-// {
-//   absHead := absHead + 1;
-// }
-
-// procedure {:layer 1} {:inline 1} intro_incrTail()
-//   modifies absTail;
-// {
-//   absTail := absTail + 1;
-// }
+procedure {:layer 1} {:inline 1} intro_writeAbsRefs(k: Key, x: Ref)
+  modifies absRefs;
+{
+  absRefs[Queue.stateTail(Queue.ofSeq(lin))] := x;
+}
 
 
 // ---------- Introduction actions:
@@ -504,12 +502,12 @@ procedure {:atomic} {:layer 2} atomic_pop() returns (k: Key)
   var {:linear "this"} this: Invoc; var my_vis: SetInvoc;
   assume Queue.pop == invoc_m(this);
 
-  // Get satisfies its functional spec  // TODO check how Michael did this
+  // Satisfies its functional spec  // TODO check how Michael did this
   assume k == Queue.stateArray(Queue.ofSeq(lin))[Queue.stateHead(Queue.ofSeq(lin))];
 
   lin := Seq_append(lin, this);
   vis[this] := my_vis;
-  // Get is complete -- TODO make predicate  // TODO only writes in lin?
+  // Is complete -- TODO make predicate  // TODO only writes in lin?
   assume my_vis == Set_ofSeq(lin);
 }
 
@@ -561,34 +559,11 @@ procedure {:yields} {:layer 1} {:refines "atomic_pop"} pop() returns (k: Key)
 
       call g := casHeadTransfer(h, hn);
       if (g) {
-        // Linearization point. TODO
+        // Linearization point.
         call intro_writeLin(this);
         call my_vis := intro_readLin();
         call intro_write_vis(this, my_vis);
 
-  assert {:layer 1} Btwn(next, head, head, null);
-  assert {:layer 1} (forall x: Ref :: {queueFP[x]}{Btwn(next, head, x, null)}
-    queueFP[x] <==> (Btwn(next, head, x, null) && x != null));
-  // Tail is on that list
-  assert {:layer 1} Btwn(next, head, tail, null) && tail != null;
-  // There is also a list from start to head // TODO try just lseg(c, head)
-  assert {:layer 1} Btwn(next, start, start, head);
-  assert {:layer 1} (forall x: Ref :: {usedFP[x]}{Btwn(next, start, x, head)}
-    usedFP[x] <==> (Btwn(next, start, x, head) && x != head));
-  // Relate abstract state to concrete state:
-  assert {:layer 1} (forall i: int :: {absRefs[i]}
-    i < 0 || Queue.stateTail(Queue.ofSeq(lin)) < i <==> absRefs[i] == null);
-  assert {:layer 1} absRefs[Queue.stateHead(Queue.ofSeq(lin))] == head;
-  assert {:layer 1} (forall i: int :: {next[absRefs[i]]} absRefs[i + 1] == next[absRefs[i]]);
-  assert {:layer 1} (forall i: int :: {Queue.stateArray(Queue.ofSeq(lin))[i], data[absRefs[i]]}
-    Queue.stateArray(Queue.ofSeq(lin))[i] == data[absRefs[i]]);
-  assert {:layer 1} (forall y: Ref :: {Btwn(next, head, y, null), next[y]}
-    Btwn(next, head, y, null) && next[y] == null
-    ==> y == absRefs[Queue.stateTail(Queue.ofSeq(lin))]);
-  // Used to infer that invocations don't modify vis after they've returned
-  assert {:layer 1} (forall n1, n2 : Invoc :: called[n1] && hb(n2, n1) ==> returned[n2]);
-  // To establish precondition of intro_writeLin
-  assert {:layer 1} (forall n: Invoc :: returned[n] ==> Seq_elem(n, lin));
         break;
       }
     }  // TODO return EMPTY?
@@ -596,14 +571,26 @@ procedure {:yields} {:layer 1} {:refines "atomic_pop"} pop() returns (k: Key)
     assert {:layer 1} Inv(queueFP, usedFP, start, head, tail, next, data, lin, vis, absRefs, called, returned) && inProgress(called, returned, this);
   }
   yield;
-  assert {:expand} {:layer 1} Inv(queueFP, usedFP, start, head, tail, next, data, lin, vis, absRefs, called, returned);
+  assert {:layer 1} Inv(queueFP, usedFP, start, head, tail, next, data, lin, vis, absRefs, called, returned) && inProgress(called, returned, this) && Seq_elem(this, lin);
+  call spec_return(this);
+  yield;
+  assert {:layer 1} Inv(queueFP, usedFP, start, head, tail, next, data, lin, vis, absRefs, called, returned);
 }
 
-/*
-
-procedure {:atomic} {:layer 2} atomic_push(k: Key, x: Ref, {:linear_in "FP"} xFP: [Ref]bool)
-  // modifies absArray, absTail, absRefs;
+procedure {:atomic} {:layer 2} atomic_push(k: Key, x: Ref,
+    {:linear_in "FP"} xFP: [Ref]bool)
+  modifies lin, vis;
 {
+  var {:linear "this"} this: Invoc; var my_vis: SetInvoc;
+  assume Queue.push == invoc_m(this) && k == invoc_k(this);
+
+  // Satisfies its functional spec
+  assume true;
+
+  lin := Seq_append(lin, this);
+  vis[this] := my_vis;
+  // Is complete -- TODO make predicate
+  assume my_vis == Set_ofSeq(lin);
 }
 
 procedure {:yields} {:layer 1} {:refines "atomic_push"} push(k: Key, x: Ref,
@@ -613,6 +600,8 @@ procedure {:yields} {:layer 1} {:refines "atomic_push"} push(k: Key, x: Ref,
   requires {:layer 1} Inv(queueFP, usedFP, start, head, tail, next, data, lin, vis, absRefs, called, returned);
   ensures {:layer 1} Inv(queueFP, usedFP, start, head, tail, next, data, lin, vis, absRefs, called, returned);
 {
+  var {:linear "this"} this: Invoc;
+  var {:layer 1} my_vis: SetInvoc;
   var t, tn: Ref;
   var g: bool;
   var {:linear "FP"} tFP: [Ref]bool;
@@ -621,15 +610,21 @@ procedure {:yields} {:layer 1} {:refines "atomic_push"} push(k: Key, x: Ref,
   assert {:layer 1} Inv(queueFP, usedFP, start, head, tail, next, data, lin, vis, absRefs, called, returned);
   assert {:layer 1} !Btwn(next, head, x, null);
   assert {:layer 1} xFP[x] && next[x] == null && data[x] == k;
+
+  call this := spec_call(Queue.push, k);
+  yield;
+  assert {:layer 1} Inv(queueFP, usedFP, start, head, tail, next, data, lin, vis, absRefs, called, returned) && inProgress(called, returned, this);
+  assert {:layer 1} !Btwn(next, head, x, null);
+  assert {:layer 1} xFP[x] && next[x] == null && data[x] == k;
   tFP := xFP;
   while (true)
-    invariant {:layer 1} Inv(queueFP, usedFP, start, head, tail, next, data, lin, vis, absRefs, called, returned);
+    invariant {:layer 1} Inv(queueFP, usedFP, start, head, tail, next, data, lin, vis, absRefs, called, returned) && inProgress(called, returned, this);
     invariant {:layer 1} !Btwn(next, head, x, null);
     invariant {:layer 1} tFP == xFP && xFP[x] && next[x] == null && data[x] == k;
   {
     call t := readTail();
     yield;
-    assert {:layer 1} Inv(queueFP, usedFP, start, head, tail, next, data, lin, vis, absRefs, called, returned);
+    assert {:layer 1} Inv(queueFP, usedFP, start, head, tail, next, data, lin, vis, absRefs, called, returned) && inProgress(called, returned, this);
     assert {:layer 1} !Btwn(next, head, x, null);
     assert {:layer 1} tFP == xFP && xFP[x] && next[x] == null && data[x] == k;
     assert {:layer 1} t != null && (queueFP[t] || usedFP[t]);
@@ -637,7 +632,7 @@ procedure {:yields} {:layer 1} {:refines "atomic_push"} push(k: Key, x: Ref,
 
     call tn := readNext(t);
     yield;
-    assert {:layer 1} Inv(queueFP, usedFP, start, head, tail, next, data, lin, vis, absRefs, called, returned);
+    assert {:layer 1} Inv(queueFP, usedFP, start, head, tail, next, data, lin, vis, absRefs, called, returned) && inProgress(called, returned, this);
     assert {:layer 1} !Btwn(next, head, x, null);
     assert {:layer 1} tFP == xFP && xFP[x] && next[x] == null && data[x] == k;
     assert {:layer 1} t != null && (queueFP[t] || usedFP[t]);
@@ -647,23 +642,31 @@ procedure {:yields} {:layer 1} {:refines "atomic_push"} push(k: Key, x: Ref,
     if (tn == null) {
       call g, tFP := casNextTransfer(t, tn, x, tFP);
       if (g) {
-        // Linearization point. TODO
-        // call intro_incrTail();
-        call intro_writeAbs(k, x);
+        // Linearization point.
+        call intro_writeLin(this);
+        call my_vis := intro_readLin();
+        call intro_write_vis(this, my_vis);
+        call intro_writeAbsRefs(k, x);
+
         break;
       }
     } else {
       call g := casTail(t, tn);
     }
     yield;
-    assert {:layer 1} Inv(queueFP, usedFP, start, head, tail, next, data, lin, vis, absRefs, called, returned);
+    assert {:layer 1} Inv(queueFP, usedFP, start, head, tail, next, data, lin, vis, absRefs, called, returned) && inProgress(called, returned, this);
     assert {:layer 1} !Btwn(next, head, x, null);
     assert {:layer 1} tFP == xFP && xFP[x] && next[x] == null && data[x] == k;
   }
   yield;
+  assert {:layer 1} Inv(queueFP, usedFP, start, head, tail, next, data, lin, vis, absRefs, called, returned) && inProgress(called, returned, this) && Seq_elem(this, lin);
+  call spec_return(this);
+  yield;
   assert {:expand} {:layer 1} Inv(queueFP, usedFP, start, head, tail, next, data, lin, vis, absRefs, called, returned);
 }
 
+
+/*
 
 procedure {:atomic} {:layer 2} atomic_size() returns (s: int)
 {}
